theories/Tactics.v
@@ -110,11 +110,11 @@ Ltac autosubst_typeclass_normalize :=
   repeat match goal with
   | [|- context[ids ?x]] =>
     let s := constr:(ids x) in progress change (ids x) with s
-  | [|- appcontext[renV ?xi]] =>
+  | [|- context[renV ?xi]] =>
     let s := constr:(renV xi) in progress change (renV xi) with s
-  | [|- appcontext[rename ?xi]] =>
+  | [|- context[rename ?xi]] =>
     let s := constr:(rename xi) in progress change (rename xi) with s
-  | [|- appcontext[subst ?sigma]] =>
+  | [|- context[subst ?sigma]] =>
     let s := constr:(subst sigma) in progress change (subst sigma) with s
   end.
 
@@ -123,11 +123,11 @@ Ltac autosubst_typeclass_normalizeH H :=
   repeat match typeof H with
   | context[ids ?x] =>
     let s := constr:(ids x) in progress change (ids x) with s in H
-  | appcontext[renV ?xi] =>
+  | context[renV ?xi] =>
     let s := constr:(renV xi) in progress change (renV xi) with s in H
-  | appcontext[rename ?xi] =>
+  | context[rename ?xi] =>
     let s := constr:(rename xi) in progress change (rename xi) with s in H
-  | appcontext[subst ?sigma] =>
+  | context[subst ?sigma] =>
     let s := constr:(subst sigma) in progress change (subst sigma) with s in H
   end.
 
@@ -150,6 +150,13 @@ Ltac autosubst_unfoldG :=
   repeat (unfold subst1, renV, upren, updV, newV, funcompV; simpl);
   repeat match goal with [|- context[_ (?VarC ?o ?x)]] => progress change (VarC o x) with (Var o x) end.
 
+Ltac autosubst_unfoldH H :=
+  autosubst_typeclass_normalizeH H; autosubst_unfold_upH H;
+  rewrite ?(@rename_substX _ _ _ _ _ _) in H;
+  repeat (unfold subst1, renV, upren, updV, newV, funcompV in H; simpl in H);
+  repeat match typeof H with
+         | context[_ (?VarC ?o ?x)] => progress change (VarC o x) with (Var o x) in H end.
+
 (* Ltac autosubst_unfoldH H := *)
 (*   autosubst_typeclass_normalizeH H; autosubst_unfold_upH H; *)
 (*   rewrite ?(@rename_substX _ _ _ _ _ _) in H; unfold renV, upren, newV in H. *)
@@ -171,52 +178,196 @@ Ltac autosubst_foldG :=
   repeat match goal with |- context[@Var _ _ ?VarC ?o ?x] => change (@Var _ _ VarC o x) with (VarC o x); try unfold VarC end;
   repeat match goal with |- context[?f >> DOM ?R] => change (f >> DOM R) with (DOM f >> R) end.
 
+Ltac autosubst_foldH H :=
+  rewrite ?fold_comp_ren, ?fold_ren_cons in H;
+  repeat match typeof H with
+         | context[ ?t ] =>
+           match t with ?s.|[?sigma] =>
+                        let rec findarg sigma :=
+                            first[ replace t with s.[sigma] in H by reflexivity
+                                 | match sigma with (?sigma1, ?sigma2) =>
+                                                    first[replace t with s.[sigma1] in H by reflexivity
+                                                         | findarg sigma2]
+                                   end]
+                        in
+                        findarg sigma
+           end end;
+  repeat match typeof H with
+         | context[@Var _ _ ?VarC ?o ?x] => change (@Var _ _ VarC o x) with (VarC o x) in H; try unfold VarC in H end;
+  repeat match typeof H with
+         | context[?f >> DOM ?R] => change (f >> DOM R) with (DOM f >> R) in H end.
+
 Ltac etaReduce := repeat lazymatch goal with [|- context[fun x => ?f x]] => change (fun x => f x) with f end.
 
 Ltac etaReduceH H := repeat lazymatch goal with [H : context[fun x => ?f x] |- _ ] => change (fun x => f x) with f in H end.
 
 (* What is all that folding and unfolding about ? *)
 Ltac autosubst_normalizeG :=
-  fsimplG; try
+  fsimplG; rel_stepG; try
   let subst_idX_inst := fresh "E" in
-    lazymatch goal with [|- appcontext[@subst _ _ _ ?Subst_term]] =>
+    lazymatch goal with [|- context[@subst _ _ _ ?Subst_term]] =>
     pose proof (@subst_idX _ _ _ _ _ Subst_term _) as subst_idX_inst;
     unfold newV in subst_idX_inst;
     simpl in subst_idX_inst
   end; repeat first
   [ progress (
-      autosubst_unfoldG; fsimpl; autosubst_unfold_up; (* ??? why *)
+      autosubst_unfoldG; fsimplG; rel_stepG; autosubst_unfold_up;
       autorewrite with autosubst;
       rewrite ?id_scompX, ?id_scompR, ?subst_compX,
-      ?subst_compR, ?id_subst, ?subst_id, ?subst_compI, ?subst_idX_inst,
-      ?rapp_eq1, ?rapp_eq2, ?rapp_rapp, ?eq_rapp, ?rapp_ex, ?ex_True
-      (* repeat match goal with [|- appcontext[@subst ?sort ?vec ?term ?Subst ?sigma]] => *)
-      (*                        replace (@subst sort vec term Subst sigma ) with (fun o : sort =>  @id (term o)) by eauto using subst_idX end *)
+      ?subst_compR, ?id_subst, ?subst_id, ?subst_compI, ?subst_idX_inst
     )
   | fold_id]; clear subst_idX_inst
 .
 
+Ltac autosubst_normalizeH H :=
+  fsimplH H; rel_stepH H; try
+  let subst_idX_inst := fresh "E" in
+    lazymatch typeof H with | context[@subst _ _ _ ?Subst_term] =>
+    pose proof (@subst_idX _ _ _ _ _ Subst_term _) as subst_idX_inst;
+    unfold newV in subst_idX_inst;
+    simpl in subst_idX_inst
+end; repeat first
+  [ progress (
+      autosubst_unfoldH H; fsimplH H; rel_stepH H; autosubst_unfold_upH H;
+      autorewrite with autosubst in H;
+      rewrite ?id_scompX, ?id_scompR, ?subst_compX,
+      ?subst_compR, ?id_subst, ?subst_id, ?subst_compI, ?subst_idX_inst in H
+    )
+  | fold_idH H]; clear subst_idX_inst
+.
+
 Ltac asimplG := autosubst_unfoldG; autosubst_normalizeG; autosubst_foldG.
+Ltac asimplH H := autosubst_unfoldH H; autosubst_normalizeH H; autosubst_foldH H.
 
-(* Ltac asimplH H := *)
-(*   simpl in H; autosubst_unfoldH H; repeat first *)
-(*   [ progress ( *)
-(*         simpl in H; *)
-(*         unfold _bind, renV, funcompV in H; fsimplH H; *)
-(*         autosubst_unfold_upH H; *)
-(*         autorewrite with autosubst in H; *)
-(*         rewrite ?id_scompX, ?id_scompR, ?subst_compX, *)
-(*         (* ?subst_compR, *) ?id_subst, ?subst_id in H; *)
-(*         repeat setoid_rewrite subst_compI in H; *)
-(*         let E := constr:(@subst_idX _ _ _ _ _ _) in rewrite ?(E _ _) in H (* I have no idea why this works ... well, it does no longer in Coq 8.5*) *)
-(*       ) *)
-(*   | fold_idH H](* ; *) *)
-(* (* fold_ren; fold_comp; fold_up *). *)
+(* Machinery for asimpl in hypotheses.
+  TODO: remove let hiding of evars once asimpl can do this generically. *)
 
+Lemma rbb0 (P Q : Prop) : P -> (let Q' := Q in (P -> Q')) -> Q.
+Proof. firstorder. Qed.
 
+(* the "all" prevents [eapply in] from seeing the universal binders. *)
+Lemma rbb1 {A : Type} (P Q : A -> Prop) :
+  (forall a, P a) -> (let Q' := Q in forall a, P a -> Q' a) -> all Q.
+Proof. firstorder. Qed.
+
+Lemma rbb2 {A B : Type} (P Q : A -> B -> Prop) :
+  (forall a b, P a b) -> (let Q' := Q in forall a b, P a b -> Q' a b) ->
+  all (fun a => forall b, Q a b).
+Proof. firstorder. Qed.
+
+Lemma rbb2_dep {A : Type} {B : A -> Type} (P Q : forall a : A, B a -> Prop) :
+  (forall a b, P a b) -> (let Q' := Q in forall a b, P a b -> Q' a b) ->
+  all (fun a => (forall b, Q a b)).
+Proof. firstorder. Qed.
+
+Lemma rbb3 {A B C : Type} (P Q : A -> B -> C -> Prop) :
+  (forall a b c, P a b c) ->
+  (let Q' := Q in forall a b c, P a b c -> Q' a b c) ->
+  all (fun a => (forall b c, Q a b c)).
+Proof. firstorder. Qed.
+
+Lemma rbb3_dep
+      {A : Type} {B : A -> Type} {C : forall a : A, B a -> Type}
+      (P Q : forall (a : A) (b : B a), C a b -> Prop) :
+  (forall a b c, P a b c) ->
+  (let Q' := Q in forall a b c, P a b c -> Q' a b c) ->
+  all (fun a => (forall b c, Q a b c)).
+Proof. firstorder. Qed.
+
+Lemma rbb4 {A B C D : Type} (P Q : A -> B -> C -> D -> Prop) :
+  (forall a b c d, P a b c d) ->
+  (let Q' := Q in forall a b c d, P a b c d -> Q' a b c d) ->
+  all (fun a => (forall b c d, Q a b c d)).
+Proof. firstorder. Qed.
+
+Lemma rbb4_dep
+      {A : Type} {B : A -> Type} {C : forall a : A, B a -> Type} {D : forall (a : A) (b : B a), C a b -> Type}
+      (P Q : forall (a : A) (b : B a) (c : C a b), D a b c -> Prop) :
+  (forall a b c d, P a b c d) ->
+  (let Q' := Q in forall a b c d, P a b c d -> Q' a b c d) ->
+  all (fun a => (forall b c d, Q a b c d)).
+Proof. firstorder. Qed.
+
+Lemma rbb5 {A B C D E : Type} (P Q : A -> B -> C -> D -> E -> Prop) :
+  (forall a b c d e, P a b c d e) ->
+  (let Q' := Q in forall a b c d e, P a b c d e -> Q' a b c d e) ->
+  all (fun a => (forall b c d e, Q a b c d e)).
+Proof. firstorder. Qed.
+
+Lemma rbb5_dep
+      {A : Type}
+      {B : A -> Type}
+      {C : forall a : A, B a -> Type}
+      {D : forall (a : A) (b : B a), C a b -> Type}
+      {E : forall (a : A) (b : B a) (c : C a b), D a b c -> Type}
+      (P Q : forall (a : A) (b : B a) (c : C a b) (d : D a b c), E a b c d -> Prop) :
+  (forall a b c d e, P a b c d e) ->
+  (let Q' := Q in forall a b c d e, P a b c d e -> Q' a b c d e) ->
+  all (fun a => (forall b c d e, Q a b c d e)).
+Proof. firstorder. Qed.
+
+Lemma rbb6 {A B C D E F : Type} (P Q : A -> B -> C -> D -> E -> F -> Prop) :
+  (forall a b c d e f, P a b c d e f) ->
+  (let Q' := Q in forall a b c d e f, P a b c d e f -> Q' a b c d e f) ->
+  all (fun a => (forall b c d e f, Q a b c d e f)).
+Proof. firstorder. Qed.
+
+Lemma rbb6_dep
+      {A : Type}
+      {B : A -> Type}
+      {C : forall a : A, B a -> Type}
+      {D : forall (a : A) (b : B a), C a b -> Type}
+      {E : forall (a : A) (b : B a) (c : C a b), D a b c -> Type}
+      {F : forall (a : A) (b : B a) (c : C a b) (d : D a b c), E a b c d -> Type}
+      (P Q : forall (a : A) (b : B a) (c : C a b) (d : D a b c) (e : E a b c d), F a b c d e -> Prop) :
+  (forall a b c d e f, P a b c d e f) ->
+  (let Q' := Q in forall a b c d e f, P a b c d e f -> Q' a b c d e f) ->
+  all (fun a => (forall b c d e f, Q a b c d e f)).
+Proof. firstorder. Qed.
+
+Lemma rbb7 {A B C D E F G : Type} (P Q : A -> B -> C -> D -> E -> F -> G -> Prop) :
+  (forall a b c d e f g, P a b c d e f g) ->
+  (let Q' := Q in forall a b c d e f g, P a b c d e f g -> Q' a b c d e f g) ->
+  all (fun a => (forall b c d e f g, Q a b c d e f g)).
+Proof. firstorder. Qed.
+
+Lemma rbb8 {A B C D E F G H : Type} (P Q : A -> B -> C -> D -> E -> F -> G -> H -> Prop) :
+  (forall a b c d e f g h, P a b c d e f g h) ->
+  (let Q' := Q in forall a b c d e f g h, P a b c d e f g h -> Q' a b c d e f g h) ->
+  all (fun a => (forall b c d e f g h, Q a b c d e f g h)).
+Proof. firstorder. Qed.
+
+Lemma rbb9 {A B C D E F G H I : Type} (P Q : A -> B -> C -> D -> E -> F -> G -> H -> I -> Prop) :
+  (forall a b c d e f g h i, P a b c d e f g h i) ->
+  (let Q' := Q in forall a b c d e f g h i, P a b c d e f g h i -> Q' a b c d e f g h i) ->
+  all (fun a => (forall b c d e f g h i, Q a b c d e f g h i)).
+Proof. firstorder. Qed.
+
+Lemma rbb10 {A B C D E F G H I J: Type} (P Q : A -> B -> C -> D -> E -> F -> G -> H -> I -> J -> Prop) :
+  (forall a b c d e f g h i j, P a b c d e f g h i j) ->
+  (let Q' := Q in forall a b c d e f g h i j, P a b c d e f g h i j -> Q' a b c d e f g h i j) ->
+  all (fun a => (forall b c d e f g h i j, Q a b c d e f g h i j)).
+Proof. firstorder. Qed.
+
+Ltac asimplHQ H :=
+  lazymatch typeof H with
+  | (forall a b c d e f g h i j, (@?T a b c d e f g h i j)) => eapply (@rbb10 _ _ _ _ _ _ _ _ _ _ T) in H
+  | (forall a b c d e f g h i, (@?T a b c d e f g h i)) => eapply (@rbb9 _ _ _ _ _ _ _ _ _ T) in H
+  | (forall a b c d e f g h, (@?T a b c d e f g h)) => eapply (@rbb8 _ _ _ _ _ _ _ _ T) in H
+  | (forall a b c d e f g, (@?T a b c d e f g)) => eapply (@rbb7 _ _ _ _ _ _ _ T) in H
+  | (forall a b c d e f, (@?T a b c d e f)) => eapply (@rbb6_dep _ _ _ _ _ _ T) in H
+  | (forall a b c d e, (@?T a b c d e)) => eapply (@rbb5_dep _ _ _ _ _ T) in H
+  | (forall a b c d, (@?T a b c d)) => eapply (@rbb4_dep _ _ _ _ T) in H
+  | (forall a b c, (@?T a b c)) => eapply (@rbb3_dep _ _ _ T) in H
+  | (forall a b, (@?T a b)) => eapply (@rbb2_dep _ _ T) in H
+  | (forall a, (@?T a)) => eapply (@rbb1 _ T) in H
+  | ?T  => eapply (@rbb0 T) in H
+  end;
+  [|intros; lazymatch goal with H : _ |- _ => revert H end; asimplG; exact id]; unfold all in H.
 
 Ltac asimpl := under_intros idtac (*TODO: asimplH *) asimplG.
-(*Tactic Notation "asimpl" "in" ident(H) := asimplH H. *)
+Tactic Notation "asimpl" "in" ident(H) := asimplH H.
+
 Tactic Notation "asimpl" "in" "*" := asimplG;
   let m := fresh "marker" in
   pose (m := tt); intros;
